BB_generation.v
@@ -208,7 +208,7 @@ Fixpoint cmd_BB_gen (c: cmd) (BBs: list BasicBlock)(BB_now: BasicBlock) (BB_num:
       |}
     |} in
     
-    let BB_pre_generated_results := list_cmd_BB_gen cmd_BB_gen pre (BBs++[BB_now']) BB_pre BB_num1 in
+    let BB_pre_generated_results := list_cmd_BB_gen cmd_BB_gen pre [] BB_pre BB_num1 in
 
     let BB_num2 := BB_pre_generated_results.(next_block_num) in
 
@@ -223,7 +223,7 @@ Fixpoint cmd_BB_gen (c: cmd) (BBs: list BasicBlock)(BB_now: BasicBlock) (BB_num:
       |}
     |} in
 
-    let BB_body_generated_results := list_cmd_BB_gen cmd_BB_gen body (to_result(BB_pre_generated_results)) BB_body BB_num2 in
+    let BB_body_generated_results := list_cmd_BB_gen cmd_BB_gen body [] BB_body BB_num2 in
     
     let BB_num3 := BB_body_generated_results.(next_block_num) in
 
@@ -233,7 +233,7 @@ Fixpoint cmd_BB_gen (c: cmd) (BBs: list BasicBlock)(BB_now: BasicBlock) (BB_num:
       jump_info := BB_now.(jump_info)
     |} in
       
-    {| BasicBlocks := to_result(BB_pre_generated_results) ; 
+    {| BasicBlocks := BBs ++ BB_now' :: nil ++ to_result(BB_pre_generated_results) ++ to_result(BB_body_generated_results); 
       BBn := BB_next;
        next_block_num := BB_num3 |}
   end.
